More examples (+ weakening and subdirectionning ; missing cases for conversion)

theories/DirectedDeclarativeTyping.v
@@ -56,12 +56,13 @@ with WfTypeDecl  : context -> direction -> term -> Type :=
     | wfTypeU {Γ d} :
         [ |-( ) Γ ] ->
         [ Γ |-( d ) U ]
-    | wfTypeProd {Γ d} {A B} :
-        [ Γ |-( dir_op d ) A ] ->
-        [Γ ,, Discr \ A @ dir_op d |-( d ) B ] ->
-        [ Γ |-( d ) tProd A B ]
-    | wfTypeUniv {Γ d} {A} :
-        [ Γ |-( d ) A : U @( Discr ) ] ->
+    | wfTypeProd {Γ A dA B dB dT} :
+        [ Γ |-( dA ) A ] ->
+        [Γ ,, Discr \ A @ dA |-( dB ) B ] ->
+        max_dir (dir_op dA) dB dT ->
+        [ Γ |-( dT ) tProd A B ]
+    | wfTypeUniv {Γ d dU} {A} :
+        [ Γ |-( d ) A : U @( dU ) ] ->
         [ Γ |-( d ) A ]
 (** **** Typing *)
 with TypingDecl : context -> direction -> term -> direction -> term -> Type :=
@@ -70,18 +71,21 @@ with TypingDecl : context -> direction -> term -> direction -> term -> Type :=
         in_ctx Γ n (d \ T @ dT) ->
         dir_leq d d' ->
         [ Γ |-( d' ) tRel n : T @( dT ) ]
-    | wfTermProd {Γ d} {A B} :
-        [ Γ |-( dir_op d ) A : U @( Discr ) ] ->
-        [Γ ,, Discr \ A @ dir_op d |-( d ) B : U @( Discr ) ] ->
-        [ Γ |-( d ) tProd A B : U @( Discr ) ]
+    | wfTermProd {Γ A dA B dB dT} :
+        [ Γ |-( dA ) A : U @( Discr ) ] ->
+        [Γ ,, Discr \ A @ dA |-( dB ) B : U @( Discr ) ] ->
+        max_dir (dir_op dA) dB dT ->
+        [ Γ |-( dT ) tProd A B : U @( Discr ) ]
     | wfTermLam {Γ d} {dT A B t} :
         [ Γ |-( dir_op dT ) A ] ->
-        [ Γ ,, Discr \ A @ dT |-( d ) t : B @( dT ) ] ->
+        [ Γ ,, Discr \ A @ dir_op dT |-( d ) t : B @( dT ) ] ->
         [ Γ |-( d ) tLambda A t : tProd A B @( dT ) ]
-    | wfTermApp {Γ d} {dT f a A B} :
+    | wfTermApp {Γ d} {dT dB f a A B} :
         [ Γ |-( d ) f : tProd A B @( dT ) ] ->
         [ Γ |-( Discr ) a : A @( dir_op dT ) ] ->
-        [ Γ |-( d ) tApp f a : B[a..] @( dT ) ]
+        [ Γ |-(dir_op dT) A ] ->
+        [ Γ ,, Discr \ A @ dir_op dT |-(dB) B] ->
+        [ Γ |-( d ) tApp f a : B[a..] @( dB ) ]
     | wfTermConv {Γ d} {t dA A B} :
         [ Γ |-( d ) t : A @( dA ) ] ->
         [ Γ |-( dA ) A ≅ B ] ->
@@ -149,17 +153,6 @@ and   "[ Γ |-( dt ) t : T @( dT ) ]" := (TypingDecl Γ dt T dT t)
 and   "[ Γ |-( d ) A ≅ B ]" := (ConvTypeDecl Γ d A B)
 and   "[ Γ |-( dt ) t ≅ t' : T @( dT ) ]" := (ConvTermDecl Γ dt T dT t t').
 
-#[local]
-Example var_fun : [ εᵈ ,, Discr \ U @ Discr |-( Fun ) tRel 0 ].
-Proof.
-  constructor.
-  econstructor.
-  - repeat constructor.
-  - constructor.
-  - constructor.
-Qed.
-
-
 (** ** Induction principles *)
 
 (** We use Scheme to generate mutual induction principle. Sadly, Scheme uses
@@ -216,3 +209,485 @@ Definition WfDeclInductionConcl :=
 End InductionPrinciples.
 
 Arguments WfDeclInductionConcl PCon PTy PTm PTyEq PTmEq : rename.
+
+
+Section Weakening.
+
+  Inductive WellDirWeakening : forall (Γ Δ : context), (nat -> nat) -> Type :=
+  | wellDirWkEmpty ρ : WellDirWeakening εᵈ εᵈ ρ
+  | wellDirWkStep Γ Δ A ρ :
+    WellDirWeakening Γ Δ ρ -> WellDirWeakening (Γ ,, A) Δ (ρ >> S) 
+  | wellDirWkUp Γ Δ d d' dA (* TODO : dA' *) A ρ :
+    dir_leq d d' ->
+    WellDirWeakening Γ Δ ρ -> 
+    WellDirWeakening (Γ ,, (d \ A @ dA)⟨ρ⟩) (Δ ,, d' \ A @ dA) (up_ren ρ).
+
+  #[projections(primitive)]
+  Record DirWeakening {Γ Δ} := 
+    { dir_wk_ren :> nat -> nat ; dir_wk_well : WellDirWeakening Γ Δ dir_wk_ren }.
+
+  Arguments DirWeakening _ _ : clear implicits.
+
+  Notation "Γ ≤ Δ" := (DirWeakening Γ Δ) (at level 40).
+
+  #[global] 
+  Instance Ren1_well_dir_wk {Y Z : Type} `{Ren1 (nat -> nat) Y Z} {Γ Δ : context} :
+    (Ren1 (Γ ≤ Δ) Y Z) :=
+    fun ρ t => t⟨ρ.(dir_wk_ren)⟩.
+
+  Lemma dir_wk_step {Γ Δ} A (ρ : Γ ≤ Δ) : Γ ,, A ≤ Δ.
+  Proof. do 2 econstructor; now eapply dir_wk_well. Unshelve. tea. Defined.
+  
+  Lemma dir_wk_up {Γ Δ} A (ρ : Γ ≤ Δ) : Γ ,, A⟨ρ⟩ ≤ Δ ,, A.
+  Proof.
+    econstructor; eapply wellDirWkUp.
+    1:reflexivity.
+    now eapply dir_wk_well.
+  Defined.
+
+  Lemma dir_wk_id_mut Γ : ∑ (ρ : Γ ≤ Γ), ρ =1 id. 
+  Proof.
+    induction Γ.
+    - unshelve econstructor.
+      + unshelve econstructor.
+        1: exact id.
+        econstructor.
+      + intros; reflexivity.
+    - destruct IHΓ as [ρ eq].
+      unshelve econstructor.
+      + unshelve econstructor.
+        1: exact (up_ren ρ).
+        assert (eqa : a = a⟨ρ⟩).
+        1: destruct a; cbn; f_equal; rewrite eq; now asimpl.
+        rewrite {1}eqa.
+        econstructor; [reflexivity| eapply dir_wk_well].
+      + intros []; cbn; first reflexivity; now rewrite eq.
+  Qed.
+
+  Lemma dir_wk_id Γ : Γ ≤ Γ.
+  Proof. apply dir_wk_id_mut. Defined.
+
+  Lemma dir_wk_id_eq Γ : dir_wk_id Γ =1 id.
+  Proof. unfold dir_wk_id; now destruct (dir_wk_id_mut Γ). Qed.
+
+  Lemma dir_wk1 Γ A : Γ ,, A ≤ Γ.
+  Proof. eapply dir_wk_step; eapply dir_wk_id. Defined.
+
+  Lemma dir_wk1_eq Γ A : dir_wk1 Γ A =1 ↑.
+  Proof. intros ?; cbn; now rewrite dir_wk_id_eq. Qed.
+
+  Lemma dir_wk_pointwise_tm {Γ Δ} (ρ : Γ ≤ Δ) (τ : nat -> nat) :
+    ρ =1 τ -> forall (t : term), t⟨ρ⟩ = t⟨τ⟩.
+  Proof.
+    intros eq ?; change ?t⟨?ρ⟩ with t⟨ρ.(dir_wk_ren)⟩ at 1; now rewrite eq.
+  Qed.
+
+  Lemma dir_wk_pointwise {Γ Δ} (ρ : Γ ≤ Δ) (τ : nat -> nat) :
+    ρ =1 τ -> forall t, t⟨ρ⟩ = t⟨τ⟩.
+  Proof.
+    intros eq []; cbn; f_equal; now rewrite eq.
+  Qed.
+
+  Lemma dir_wk1_ren_on Γ A (t : term) : t⟨↑⟩ = t⟨dir_wk1 Γ A⟩.
+  Proof. 
+    erewrite <-dir_wk_pointwise_tm; first reflexivity.
+    eapply dir_wk1_eq.
+  Qed.
+
+  Lemma dir_wk_in_ctx {Γ Δ} (ρ : Δ ≤ Γ) : forall {A n}, in_ctx Γ n A -> ∑ d', dir_leq d' A.(dir) × in_ctx Δ (ρ n) (d' \ A.(ty)⟨ρ⟩ @ A.(ty_dir)).
+  Proof.
+    destruct ρ as [ρ wρ]; induction wρ; cbn; intros B n hin.
+    all: change (ty ?A)⟨{| dir_wk_ren := ?ρ ; dir_wk_well := _ |}⟩ with (ty A)⟨ρ⟩.
+    - inversion hin.
+    - replace (ty B)⟨_⟩ with (ty B)⟨ρ⟩⟨↑⟩ by now asimpl.
+      destruct (IHwρ _ _ hin) as [? []].
+      eexists; split; tea.
+      change (?d \ ?A⟨↑⟩ @ ?dA) with (d \ A @ dA)⟨↑⟩.
+      now econstructor.
+    - destruct n as [|m]; cbn.
+      + inversion hin; subst.
+        eexists; split; tea.
+        cbn; replace (_ \ _⟨_⟩⟨_⟩ @ _) with (d \ A⟨ρ⟩ @ dA)⟨↑⟩.
+        2: cbn; f_equal; cbn; asimpl; reflexivity.
+        econstructor.
+      + inversion hin; subst.
+        destruct (IHwρ _ _ H3) as [dB []].
+        eexists; destruct d1 as [B Bdir ?]; split; tea; cbn.
+        replace (_ \ _⟨_⟩⟨_⟩ @ _) with (dB \ B⟨ρ⟩ @ Bdir)⟨↑⟩.
+        2: cbn; f_equal; cbn; asimpl; reflexivity.
+        now econstructor.
+  Qed.
+        
+
+  Let PCon (Γ : context) := True.
+  Let PTy Γ dA A := forall Δ (ρ : Δ ≤ Γ), [|-() Δ] -> [Δ |-(dA) A⟨ρ⟩].
+  Let PTm Γ d A dA t := forall Δ (ρ : Δ ≤ Γ), [|-() Δ] -> [Δ |-(d) t⟨ρ⟩ : A⟨ρ⟩ @(dA)].
+  Let PTyEq Γ dA A B := forall Δ (ρ : Δ ≤ Γ), [|-() Δ] -> [Δ |-(dA) A⟨ρ⟩ ≅ B⟨ρ⟩].
+  Let PTmEq Γ d A dA t u := forall Δ (ρ : Δ ≤ Γ), [|-() Δ] -> [Δ |-(d) t⟨ρ⟩ ≅ u⟨ρ⟩ : A⟨ρ⟩ @(dA)].
+  
+  Theorem dir_wk : WfDeclInductionConcl PCon PTy PTm PTyEq PTmEq.
+  Proof.
+    apply WfDeclInduction; try (intros; exact I).
+    - intros ** ???; cbn; now constructor.
+    - intros * ? ihA ? ihB ???. cbn. 
+      econstructor; tea.
+      1: now eapply ihA.
+      change B⟨_⟩ with B⟨dir_wk_up (Discr \ A @ dA) ρ⟩.
+      eapply ihB.
+      econstructor; tea; now eapply ihA.
+    - intros * ? ihU ???; econstructor.
+      change U with U⟨ρ⟩; eapply ihU; tea.
+    - intros ** ???; cbn.
+      apply (dir_wk_in_ctx ρ) in H0 as [d'' []].
+      econstructor; tea.
+      now etransitivity.
+    - intros * ? ihA ? ihB ???.
+      econstructor; tea; change U with U⟨ρ⟩.
+      1: now apply ihA.
+      change B⟨_⟩ with B⟨dir_wk_up (Discr \ A @ dA) ρ⟩.
+      apply ihB.
+      econstructor; tea; econstructor; now eapply ihA.
+    - intros * ? ihA ? iht ???.
+      econstructor.
+      1: now eapply ihA.
+      change ?t⟨upRen_term_term _⟩ with t⟨dir_wk_up (Discr \ A @ dir_op dT) ρ⟩.
+      eapply iht; econstructor; tea. 
+      now eapply ihA.
+    - intros * ? ihf ? iha ? ihA ? ihB ???.
+      replace B[a..]⟨ρ⟩ with B⟨up_ren ρ⟩[a⟨ρ⟩..].
+      2: destruct ρ; cbn; asimpl; reflexivity.
+      econstructor.
+      + replace (tProd _ _) with (tProd A B)⟨ρ⟩.
+        2: cbn; f_equal.
+        now eapply ihf.
+      + now eapply iha.
+      + now eapply ihA.
+      + eapply (ihB _ (dir_wk_up (Discr \ A @ dir_op dT) ρ)).
+        econstructor; tea.
+        now eapply ihA.
+    - intros * ? iht ? ihAB ???.
+      econstructor.
+      1: now eapply iht.
+      now eapply ihAB.
+    - admit.
+    - admit.
+    - admit.
+    - admit.
+    - admit.
+    - admit.
+    - admit.
+    - admit.
+    - admit.
+  Admitted.
+
+End Weakening.
+
+Section Subdirectionning.
+  Let PCon (Γ : context) := True.
+  Let PTy Γ dA A := forall dA', dA ⪯ dA' -> [Γ |-(dA') A]. 
+  (* Need to strenghen variable cases for more subdirectionning *)
+  Let PTm Γ d A dA t := forall d' , d ⪯ d' -> (* dA ⪯ dA' -> *) [Γ |-(d') t : A @(dA)].
+  Let PTyEq Γ dA A B := forall dA', dA ⪯ dA' -> [Γ |-(dA') A ≅ B].
+  Let PTmEq Γ d A dA t u := forall d' , d ⪯ d' -> (* dA ⪯ dA' -> *) [Γ |-(d') t ≅ u : A @(dA)].
+ 
+  Lemma subdir : WfDeclInductionConcl PCon PTy PTm PTyEq PTmEq.
+  Proof.
+    apply WfDeclInduction; try (intros; exact I). 
+    all: unfold PCon, PTy, PTm, PTyEq, PTmEq.
+    all: try solve [intros; now econstructor].
+    - intros * ? ihA ? ihB ? dT' hdT'; econstructor.
+      + eapply ihA; reflexivity.
+      + eapply ihB. 
+        etransitivity; last exact hdT'.
+        now eapply MaxDirProp.upper_bound2.
+      + eapply MaxDirProp.max_left; etransitivity; tea.
+        now eapply MaxDirProp.upper_bound1.
+    - intros **. 
+      econstructor; tea.
+      now etransitivity.
+    - intros * ? ihA ? ihB ?? hdT'; econstructor. 
+      + eapply ihA; reflexivity.
+      + eapply ihB. 
+        etransitivity; last exact hdT'.
+        now eapply MaxDirProp.upper_bound2.
+      + eapply MaxDirProp.max_left; etransitivity; tea.
+        now eapply MaxDirProp.upper_bound1.
+    - intros * ? ihA ? ihAB ? ihCD ? hdT'; econstructor.
+      (* add the max in the congruence rule for products *)
+      admit.
+    Admitted.
+
+End Subdirectionning.
+
+
+(** More derived typing lemmas *)
+
+Lemma wfCtxCons' {Θ d A dA} : 
+  [|-() Θ] -> 
+  ([|-() Θ] -> [Θ |-(dA) A]) ->
+  match d with Discr => unit | _ => is_kind A end ->
+  [|-() Θ ,, d \ A @ dA].
+Proof.
+  intros hΘ hA; destruct d; econstructor; tea; eauto.
+Qed.
+
+Lemma wfTypeProd' {Γ d} {A B} :
+  [ |-() Γ  ] -> 
+  [ Γ |-( dir_op d ) A ] ->
+  ( [|-() Γ ,, Discr \ A @ dir_op d] -> 
+    [ Γ |-( dir_op d ) A ] ->
+    [Γ ,, Discr \ A @ dir_op d |-( d ) B ]) ->
+  [ Γ |-( d ) tProd A B ].
+Proof.
+  intros hΓ hA hB.
+  econstructor; tea.
+  1: apply hB; tea; now econstructor.
+  destruct d; reflexivity.
+Qed.
+
+
+Fixpoint shift_n {A} `{Ren1 (nat -> nat) A A} (t : A) n := match n with 0 => t | S m => (shift_n t m)⟨↑⟩ end.
+
+Lemma wfTypeVar {Θ n d d' dU} :
+  [ |-( ) Θ ] ->
+  in_ctx Θ n (shift_n (d \ U @ dU) n) ->
+  dir_leq d d' ->
+  [ Θ |-( d' ) tRel n ].
+Proof.
+  assert (h : forall k, shift_n (d \ U @ dU) k = (d \ U @ dU)).
+  by (intros k; induction k as [| ? ih]; cbn; rewrite ?ih; reflexivity).
+  rewrite h.
+  intros.
+  eapply wfTypeUniv.
+  now econstructor.
+Qed.
+
+
+
+Module Examples.
+
+  #[local]
+  Example var_fun : [ εᵈ ,, Discr \ U @ Discr |-( Fun ) tRel 0 ].
+  Proof.
+    eapply wfTypeVar; repeat econstructor.
+  Qed.
+
+  Module List.
+  
+  (* Context of parameters for list *)
+  Definition ctx := εᵈ ,, Fun \ U @ Discr.
+  (* Context of arguments for nil; 
+    the parameters of list should form a prefix *)
+  Definition nil_ctx := ctx.
+  (* Not sure how we will represent inductive occurences
+    of the inductive being defined so I abstract that 
+    as an arbitrary function tList taking |ctx| arguments of type term
+    and producing a term for now *)
+  Definition cons_ctx (tList : term -> term) := ctx,, Discr \ tRel 0 @ Fun,, Discr \ tList (tRel 1) @ Fun.
+
+  Section ListTyping.
+
+  Lemma ctxWfCtx : [|-() ctx ].
+  Proof. repeat econstructor. Qed.
+
+  Lemma nil_ctxWfCtx : [|-() nil_ctx ].
+  Proof.  apply ctxWfCtx.  Qed.
+
+  Lemma cons_ctxWfCtx 
+    (tList : term -> term)
+    (ih : forall Θ A, [Θ |-(Fun) A] -> [Θ |-(Fun) tList A]) :
+    [|-() cons_ctx tList ].
+  Proof.
+    pose ctxWfCtx; eapply wfCtxCons'; [econstructor|intros| easy]; tea.
+    - do 2 econstructor; tea; econstructor.
+    - eapply ih. 
+      eapply wfTypeVar; tea.
+      2: reflexivity.
+      do 2 econstructor.
+  Qed.
+
+  End ListTyping.
+  End List.
+
+
+  Module W.
+
+    Definition ctx := εᵈ ,, Fun \ U @ Discr ,, Cofun \ tProd (tRel 0) U @ Cofun.
+    
+    Definition sup_ctx 
+      (* tW should bind one variable in its second argument *)
+      (tW : term -> term -> term) :=
+      ctx ,, Discr \ tRel 1 @ Fun ,, Discr \ tProd (tApp (tRel 1) (tRel 0)) (tW (tRel 3) (tApp (tRel 3) (tRel 0))) @ Fun.
+    
+    Section WTyping.
+
+    Lemma ctxWfCtx : [|-() ctx ].
+    Proof.
+      eapply wfCtxCons'; [eapply wfCtxCons'|..]; intros.
+      1-3,5: unshelve econstructor; tea.
+      eapply wfTypeProd'; tea.
+      1: eapply wfTypeVar; [tea| repeat econstructor| reflexivity].
+      intros; now econstructor.
+    Qed.
+
+    Lemma supWfCtx (tW : term -> term -> term) 
+      (ih : forall Θ A B, 
+        [Θ |-(Fun) A] ->
+        [Θ ,, Discr \ A @ Fun |-(Cofun) B ] ->
+        [Θ |-(Fun) tW A B]) :
+      [|-() sup_ctx tW ].
+    Proof.
+      eapply wfCtxCons'; [eapply wfCtxCons'|..]; try easy; intros.
+      1: apply ctxWfCtx.
+      1: eapply wfTypeVar; tea; [do 2 econstructor|reflexivity].
+      eapply wfTypeProd'; intros; tea.
+      + eapply (wfTypeUniv (dU:=Cofun)).
+        change U with (U[(tRel 0)..]).
+        eapply (wfTermApp (dT := Cofun) (A:=(tRel 2))).
+        all: econstructor; tea; try reflexivity.
+        2: econstructor.
+        - change (?d \ tProd _ _ @ ?dT) with (shift_n (d \ tProd (tRel 0) U @ dT) 2).
+          do 2 econstructor.
+        - econstructor ; tea; last reflexivity.
+          change (?d \ U @ ?dT) with (shift_n (d \ U @ dT) 3).
+          repeat econstructor.
+        - econstructor; tea.
+          eapply wfTypeVar; tea.
+          1: do 3 econstructor.
+          reflexivity.
+      + set (ctx' := _,, _ ,, _).
+        assert [ctx' |-(Fun) tRel 3].
+        1:{ eapply wfTypeVar; tea; try reflexivity; repeat econstructor. }
+        assert [|-() ctx' ,, Discr \ tRel 3 @ Fun] by now econstructor.
+        apply ih; tea.
+        eapply (wfTypeUniv (dU:=Cofun)).
+        change U with (U[(tRel 0)..]).
+        eapply (wfTermApp (dT := Cofun) (A:=(tRel 4))).
+        1,2: econstructor; tea; try reflexivity.
+        2: econstructor.
+        - change (?d \ tProd _ _ @ ?dT) with (shift_n (d \ tProd (tRel 1) U @ dT) 3).
+          repeat econstructor.
+        - eapply wfTypeVar; tea; last reflexivity.
+          repeat econstructor.
+        - do 2 econstructor; tea.
+          eapply wfTypeVar; tea.
+          1: repeat econstructor.
+          reflexivity.
+    Qed.
+
+    End WTyping.
+  End W.  
+
+
+  Module Composition.
+    Definition comp_ctx := 
+      εᵈ ,, 
+      (* A : *) Cofun \ U @ Discr ,, 
+      (* B : *) Discr \ U @ Discr ,,
+      (* C : *) Fun \ U @ Discr ,,
+      (* f : *) Discr \ arr (tRel 2) (tRel 1) @ Fun ,,
+      (* g : *) Discr \ arr (tRel 2) (tRel 1) @ Fun ,,
+      (* a : *) Discr \ tRel 4 @ Cofun.
+    
+    Definition comp_tm := tApp (tRel 1) (tApp (tRel 2) (tRel 0)).
+
+    Lemma wfTypeArr {Γ A dA B dB dT} : 
+      [|-() Γ] ->
+      [Γ |-(dA) A] ->
+      [Γ |-(dB) B] ->
+      max_dir (dir_op dA) dB dT ->
+      [Γ |-(dT) arr A B].
+    Proof.
+      intros.
+      econstructor; tea.
+      rewrite (dir_wk1_ren_on Γ (Discr \ A @ dA) B).
+      eapply dir_wk; tea.
+      econstructor; tea.
+    Qed.
+
+    Lemma comp_ctxWfCtx : [ |-() comp_ctx ].
+    Proof.
+      repeat eapply wfCtxCons'; try easy; intros; try now constructor.
+      - eapply wfTypeArr; tea.
+        1,2: eapply wfTypeVar; tea;[repeat econstructor|reflexivity].
+        reflexivity.
+      - eapply wfTypeArr; tea.
+        1,2: eapply wfTypeVar; tea;[repeat econstructor|reflexivity].
+        reflexivity.
+      - eapply wfTypeVar; tea;[repeat econstructor|reflexivity].
+    Qed.
+
+    Lemma wfTermSimpleApp {Γ d} {dT dB f a A B} :
+        [|-() Γ] ->
+        [ Γ |-( d ) f : arr A B @( dT ) ] ->
+        [ Γ |-( Discr ) a : A @( dir_op dT ) ] ->
+        [ Γ |-(dir_op dT) A] ->
+        [ Γ |-(dB) B] ->
+        [ Γ |-( d ) tApp f a : B @( dB ) ].
+    Proof.
+      intros; rewrite <- (shift_subst_eq B a).
+      econstructor; tea.
+      rewrite (dir_wk1_ren_on Γ (Discr \ A @ dir_op dT) B).
+      eapply dir_wk; tea.
+      econstructor; tea.
+    Qed.
+
+    Definition a : [ comp_ctx |-(Discr) tRel 0 : tRel 5 @(Cofun) ].
+    Proof.
+      econstructor; [apply comp_ctxWfCtx| | reflexivity].
+      change (?d \ _ @ ?dT) with (shift_n (d \ tRel 4 @ dT) 1).
+      econstructor.
+    Qed.
+
+    Definition g : [ comp_ctx |-(Discr) tRel 1 : arr (tRel 4) (tRel 3) @(Fun) ].
+    Proof.
+      econstructor; [apply comp_ctxWfCtx| | reflexivity].
+      change (?d \ _ @ ?dT) with (shift_n (d \ arr (tRel 2) (tRel 1)  @ dT) 2).
+      repeat econstructor.
+    Qed.
+    
+    Definition f : [ comp_ctx |-(Discr) tRel 2 : arr (tRel 5) (tRel 4) @(Fun) ].
+    Proof.
+      econstructor; [apply comp_ctxWfCtx| | reflexivity].
+      change (?d \ _ @ ?dT) with (shift_n (d \ arr (tRel 2) (tRel 1)  @ dT) 3).
+      repeat econstructor.
+    Qed.
+
+    Definition A : [comp_ctx |-(Cofun) tRel 5].
+    Proof.
+      eapply wfTypeVar; [apply comp_ctxWfCtx| | reflexivity].
+      repeat econstructor.
+    Qed.
+    
+    Definition B : [comp_ctx |-(Discr) tRel 4].
+    Proof.
+      eapply wfTypeVar; [apply comp_ctxWfCtx| | reflexivity].
+      repeat econstructor.
+    Qed.
+
+    Definition C : [comp_ctx |-(Fun) tRel 3].
+    Proof.
+      eapply wfTypeVar; [apply comp_ctxWfCtx| | reflexivity].
+      repeat econstructor.
+    Qed.
+
+    Lemma comp_tmWfTerm : [ comp_ctx |-(Discr) comp_tm : tRel 3 @(Fun) ].
+    Proof.
+      pose comp_ctxWfCtx.
+      unfold comp_tm.
+      eapply wfTermSimpleApp; tea.
+      - eapply g.
+      - eapply wfTermSimpleApp; tea.
+        + eapply f.
+        + eapply a.
+        + eapply A.
+        + eapply subdir; first eapply B; constructor.
+      - eapply subdir; first eapply B; constructor.
+      - eapply C.
+    Qed.
+
+  End Composition.
+  
+End Examples.
+
+
